wip

proofmode/HPSim.v
@@ -58,6 +58,7 @@ Section SIM.
 			f_src f_tgt st_src st_tgt fmr
 			v_src v_tgt
 			(RET: (Own fmr ⊢ #=> I st_src st_tgt))
+			(EQ: v_src = v_tgt)
 		:
 			_hpsim hpsim f_src f_tgt (st_src, Ret v_src) (st_tgt, Ret v_tgt) fmr
 
@@ -65,7 +66,8 @@ Section SIM.
 			f_src f_tgt st_src st_tgt fmr
 			fn varg k_src k_tgt FR
       (INV: Own fmr ⊢ #=> (I st_src st_tgt ** FR))
-			(K: forall vret st_src0 st_tgt0 fmr0
+			(K: forall vret st_src0 st_tgt0 fmr0 
+					(WF: URA.wf fmr0)
           (INV: Own fmr0 ⊢ #=> (I st_src0 st_tgt0 ** FR)),
 				_hpsim hpsim true true (st_src0, k_src vret) (st_tgt0, k_tgt vret) fmr0)				
 		:
@@ -159,7 +161,7 @@ Section SIM.
 			f_src f_tgt st_src st_tgt fmr
 			iP k_src i_tgt FMR
       (CUR: Own fmr ⊢ #=> FMR)
-			(K: forall fmr0 (NEW: Own fmr0 ⊢ #=> (iP ** FMR)),
+			(K: forall fmr0 (WF: URA.wf fmr0) (NEW: Own fmr0 ⊢ #=> (iP ** FMR)),
           _hpsim hpsim true f_tgt (st_src, k_src tt) (st_tgt, i_tgt) fmr0)
 		:
 			_hpsim hpsim f_src f_tgt (st_src, trigger (Assume iP) >>= k_src) (st_tgt, i_tgt) fmr
@@ -168,7 +170,7 @@ Section SIM.
 			f_src f_tgt st_src st_tgt fmr
 			iP i_src k_tgt FMR
       (CUR: Own fmr ⊢ #=> (iP ** FMR))
-			(K: forall fmr0 (NEW: Own fmr0 ⊢ #=> FMR),
+			(K: forall fmr0 (WF: URA.wf fmr0) (NEW: Own fmr0 ⊢ #=> FMR),
           _hpsim hpsim f_src true (st_src, i_src) (st_tgt, k_tgt tt) fmr0)
 		:
 			_hpsim hpsim f_src f_tgt (st_src, i_src) (st_tgt, trigger (Assume iP) >>= k_tgt) fmr
@@ -177,7 +179,7 @@ Section SIM.
 			f_src f_tgt st_src st_tgt fmr
 			iP k_src i_tgt FMR
       (CUR: Own fmr ⊢ #=> (iP ** FMR))
-			(K: forall fmr0 (NEW: Own fmr0 ⊢ #=> FMR),
+			(K: forall fmr0 (WF: URA.wf fmr0) (NEW: Own fmr0 ⊢ #=> FMR),
           _hpsim hpsim true f_tgt (st_src, k_src tt) (st_tgt, i_tgt) fmr0)
 		:
 			_hpsim hpsim f_src f_tgt (st_src, trigger (Guarantee iP) >>= k_src) (st_tgt, i_tgt) fmr
@@ -186,7 +188,7 @@ Section SIM.
 			f_src f_tgt st_src st_tgt fmr
 			iP i_src k_tgt FMR
       (CUR: Own fmr ⊢ #=> FMR)
-			(K: forall fmr0 (NEW: Own fmr0 ⊢ #=> (iP ** FMR)),
+			(K: forall fmr0 (WF: URA.wf fmr0) (NEW: Own fmr0 ⊢ #=> (iP ** FMR)),
           _hpsim hpsim f_src true (st_src, i_src) (st_tgt, k_tgt tt) fmr0)
 		:
 			_hpsim hpsim f_src f_tgt (st_src, i_src) (st_tgt, trigger (Guarantee iP) >>= k_tgt) fmr
@@ -218,13 +220,15 @@ Section SIM.
 		(RET: forall
 				f_src f_tgt st_src st_tgt fmr
 				v_src v_tgt
-				(RET: (Own fmr ⊢ #=> I st_src st_tgt) ),
+				(RET: (Own fmr ⊢ #=> I st_src st_tgt) )
+				(EQ: v_src = v_tgt),
 				P f_src f_tgt (st_src, Ret v_src) (st_tgt, Ret v_tgt) fmr)
 		(CALL: forall
 				f_src f_tgt st_src st_tgt fmr
 				fn varg k_src k_tgt FR
 				(INV: Own fmr ⊢ #=> (I st_src st_tgt ** FR))
 				(K: forall vret st_src0 st_tgt0 fmr0
+						(WF: URA.wf fmr0) 
 						(INV: Own fmr0 ⊢ #=> (I st_src0 st_tgt0 ** FR)),
 						<<SIM: hpsim true true (st_src0, k_src vret) (st_tgt0, k_tgt vret) fmr0>> /\
 						<<IH: P true true (st_src0, k_src vret) (st_tgt0, k_tgt vret) fmr0>>),
@@ -308,7 +312,7 @@ Section SIM.
 				f_src f_tgt st_src st_tgt fmr
 				iP k_src i_tgt FMR
 				(CUR: Own fmr ⊢ #=> FMR)
-				(K: forall fmr0 (NEW: Own fmr0 ⊢ #=> (iP ** FMR)),
+				(K: forall fmr0 (WF: URA.wf fmr0) (NEW: Own fmr0 ⊢ #=> (iP ** FMR)) ,
 						<<SIM: hpsim true f_tgt (st_src, k_src tt) (st_tgt, i_tgt) fmr0>> /\
 						<<IH: P true f_tgt (st_src, k_src tt) (st_tgt, i_tgt) fmr0>>),
 				P f_src f_tgt (st_src, trigger (Assume iP) >>= k_src) (st_tgt, i_tgt) fmr)
@@ -316,7 +320,7 @@ Section SIM.
 				f_src f_tgt st_src st_tgt fmr
 				iP i_src k_tgt FMR
 				(CUR: Own fmr ⊢ #=> (iP ** FMR))
-				(K: forall fmr0 (NEW: Own fmr0 ⊢ #=> FMR),
+				(K: forall fmr0 (WF: URA.wf fmr0) (NEW: Own fmr0 ⊢ #=> FMR),
 						<<SIM: hpsim f_src true (st_src, i_src) (st_tgt, k_tgt tt) fmr0>> /\
 						<<IH: P f_src true (st_src, i_src) (st_tgt, k_tgt tt) fmr0>>),
 				P f_src f_tgt (st_src, i_src) (st_tgt, trigger (Assume iP) >>= k_tgt) fmr)
@@ -324,7 +328,7 @@ Section SIM.
 				f_src f_tgt st_src st_tgt fmr
 				iP k_src i_tgt FMR
 				(CUR: Own fmr ⊢ #=> (iP ** FMR))
-				(K: forall fmr0 (NEW: Own fmr0 ⊢ #=> FMR),
+				(K: forall fmr0 (WF: URA.wf fmr0) (NEW: Own fmr0 ⊢ #=> FMR),
 						<<SIM: hpsim true f_tgt (st_src, k_src tt) (st_tgt, i_tgt) fmr0>> /\
 						<<IH: P true f_tgt (st_src, k_src tt) (st_tgt, i_tgt) fmr0>>),
 				P f_src f_tgt (st_src, trigger (Guarantee iP) >>= k_src) (st_tgt, i_tgt) fmr)
@@ -332,7 +336,7 @@ Section SIM.
 				f_src f_tgt st_src st_tgt fmr
 				iP i_src k_tgt FMR
 				(CUR: Own fmr ⊢ #=> FMR)
-				(K: forall fmr0 (NEW: Own fmr0 ⊢ #=> (iP ** FMR)),
+				(K: forall fmr0 (WF: URA.wf fmr0) (NEW: Own fmr0 ⊢ #=> (iP ** FMR)),
 						<<SIM: hpsim f_src true (st_src, i_src) (st_tgt, k_tgt tt) fmr0>> /\
 						<<IH: P f_src true (st_src, i_src) (st_tgt, k_tgt tt) fmr0>>),
 				P f_src f_tgt (st_src, i_src) (st_tgt, trigger (Guarantee iP) >>= k_tgt) fmr)
@@ -406,60 +410,73 @@ Section SIM.
 	Lemma own_ctx a b
 			(OWN: Own a ⊢ #=> Own b)
 		:
-			forall ctx, Own (a ⋅ ctx) ⊢ #=> Own (b ⋅ ctx)
+			forall ctx, Own (ctx ⋅ a) ⊢ #=> Own (ctx ⋅ b)
 	.
 	Proof.
 		i. iIntros "[H H0]".
-		iPoseProof (OWN with "H") as "H".
+		iPoseProof (OWN with "H0") as "H0".
 		iSplitL "H"; et.
 	Qed.
 
-	Lemma updatable_own (r r': Σ)
-			(UPD: URA.updatable r r')
+	Lemma own_wf (r r': Σ)
+			(OWN: Own r ⊢ #=> Own r')
+			(WF: URA.wf r)
 		:
-			Own r ⊢ #=> Own r'
-		.
+			URA.wf r'
+	.
+	Proof. 
+		uipropall. hexploit OWN; et. refl.
+		esplits; et. des.
+		eapply URA.wf_extends; et.
+		specialize (H0 ε). rewrite ! URA.unit_id in H0.
+		et.
+	Qed.
+
+
+
+	Lemma not_wf_sat (r: Σ) (ILL: ¬ URA.wf r) P: Own r ⊢ P.
 	Proof.
-		unfold URA.updatable in *. uipropall.
-		i. exists r'.
-		esplits; et. { r_solve. }
-		i. apply UPD. revert ctx H0.
-		eapply URA.extends_updatable. et.
+		rr. uipropall. i.
+		eapply URA.wf_extends in WF; et.
+		clarify.
 	Qed.
 
 	Lemma iProp_sepconj_aux P Q r 
 			(SAT: Own r ⊢ #=> (P ** Q))
-			(WF: URA.wf r)
 		:
 			exists rp rq, (URA.updatable r (rp ⋅ rq)) /\ 
 										(Own rp ⊢ P) /\ 
 										(Own rq ⊢ Q)
 	.
 	Proof.
+		destruct (classic (URA.wf r)); cycle 1.
+		{
+			exists r, r. esplits; eauto using not_wf_sat.
+			rr. i. eapply URA.wf_mon in H0. clarify. 
+		}
+
 		uipropall.
 		hexploit SAT; et. { r_solve. }
 		i. des.
 		esplits; et; uipropall.
 		{
 			instantiate (1:= b). instantiate (1:=a).
-			unfold URA.updatable. 
-			rewrite H in H0. et.
+			unfold URA.updatable. subst. et. 
 		}
 		{
 			i. destruct P. ss.
-			hexploit H3. i.
-			eapply URA.wf_extends in H3; et.
+			hexploit H4. i.
+			eapply URA.wf_extends in H4; et.
 		}
 		{
 			i. destruct Q. ss.
-			hexploit H3. i.
-			eapply URA.wf_extends in H3; et.
+			hexploit H4. i.
+			eapply URA.wf_extends in H4; et.
 		}
 	Qed.
 
 	Lemma iProp_sepconj P Q r 
 			(SAT: Own r ⊢ #=> (P ** Q))
-			(WF: URA.wf r)
 		:
 			exists rp rq, (Own r ⊢ #=> Own (rp ⋅ rq)) /\ 
 										(Own rp ⊢ P) /\ 
@@ -467,7 +484,7 @@ Section SIM.
 	.
 	Proof.
 		eapply iProp_sepconj_aux in SAT; et. des.
-		eapply updatable_own in SAT.
+		eapply Own_Upd in SAT.
 		esplits; et. 	
 	Qed.	
 
@@ -526,10 +543,10 @@ Section SIM.
     =
 		(* interp_state (handle_hAGE_tgt) (trigger (Assume iP)) fr *)
     ('(fr, _) <- (handle_Assume iP fr);; tau;; Ret (fr, tt))
-.
-Proof.
-	unfold interp_hp_tgt, trigger. rewrite ! interp_state_vis. grind. rewrite u. et.
-Qed.
+	.
+	Proof.
+		unfold interp_hp_tgt, trigger. rewrite ! interp_state_vis. grind. rewrite u. et.
+	Qed.
 
 	Lemma interp_hp_Guarantee
       iP
@@ -539,48 +556,48 @@ Qed.
     =
 		(* interp_state (handle_hAGE_tgt) (trigger (Assume iP)) fr *)
     ('(fr', _) <- (handle_Guarantee iP fr);; tau;; Ret (fr', tt))
-.
-Proof.
-	unfold interp_hp_tgt, trigger. rewrite ! interp_state_vis. grind. rewrite u. et.
-Qed.
+	.
+	Proof.
+		unfold interp_hp_tgt, trigger. rewrite ! interp_state_vis. grind. rewrite u. et.
+	Qed.
+
+	(* Which fr to put in interp_hp_tgt & What to return *)
+	Definition interp_hp_fun (hp: Any.t -> itree hAGEs Any.t): Any.t -> itree Es Any.t :=
+		fun arg => interp_hp_tgt_fun (hp arg) ε >>= (fun '(_, x) => Ret x).
+
+
 
   Variant mk_inv  
           (I: Any.t -> Any.t -> iProp)
-    : unit -> Any.t * Any.t -> Prop :=
+    : Σ -> Any.t * Any.t -> Prop :=
   | mk_inv_intro
-      (mr_src mr_tgt: Σ) st_src st_tgt
-			(* (MR: URA.extends mr_src mr_tgt) *)
-			(* (INV: exists mr, current_iProp mr (I st_src st_tgt)) *)
-      (INV: 
-						exists mr,
+      (ctx mr_src mr_tgt: Σ) st_src st_tgt
+      (INV: exists mr,
+						<<WF: URA.wf (ctx ⋅ mr_src)>> /\
 						<<MRS: Own mr_src ⊢ #=> Own (mr ⋅ mr_tgt)>> /\
 						<<MR: Own mr ⊢ #=> (I st_src st_tgt)>>)
     :
-      mk_inv I tt (Any.pair st_src mr_src↑, Any.pair st_tgt mr_tgt↑)
+      mk_inv I ctx (Any.pair st_src mr_src↑, Any.pair st_tgt mr_tgt↑)
   .
 
-
-  Lemma hpsim_adequacy:
+  (* Lemma hpsim_adequacy:
     forall
       f_src f_tgt st_src st_tgt (fl_src0 fl_tgt0: alist string (Any.t -> itree Es Any.t)) itr_src itr_tgt
-			(mr_src mr_tgt fr_src fr_tgt fmr: Σ)
+			(ctx mr_src mr_tgt fr_src fr_tgt fmr: Σ)
       (SIM: hpsim f_src f_tgt (st_src, itr_src) (st_tgt, itr_tgt) fmr)
-			(* (FMR: fr_src ⋅ mr_src = fmr ⋅ fr_tgt ⋅ mr_tgt), *)
-			(FMR: Own (fr_src ⋅ mr_src) ⊢ #=> Own (fmr ⋅ fr_tgt ⋅ mr_tgt)),
-
-			@sim_itree unit (mk_inv I) (fun _ _ => True) fl_src0 fl_tgt0 f_src f_tgt tt 
+			(FMR: Own (fr_src ⋅ mr_src) ⊢ #=> Own (fmr ⋅ fr_tgt ⋅ mr_tgt))
+			(WF: URA.wf (ctx ⋅ fr_src ⋅ mr_src)),
+			@sim_itree Σ (mk_inv I) (fun _ _ => True) fl_src0 fl_tgt0 f_src f_tgt ctx
 			(Any.pair st_src mr_src↑, (interp_hp_tgt_fun itr_src fr_src) >>= (fun r => Ret (snd r)))
-			(Any.pair st_tgt mr_tgt↑, (interp_hp_tgt_fun itr_tgt fr_tgt) >>= (fun r => Ret (snd r))).
+			(Any.pair st_tgt mr_tgt↑, (interp_hp_tgt_fun itr_tgt fr_tgt) >>= (fun r => Ret (snd r)))
+		.
   Proof.
 		i. 
-		(* remember (Any.pair st_src mr_src↑). remember (Any.pair st_tgt mr_tgt↑). *)
 		revert_until I.
 		ginit. gcofix CIH. i.
 		remember (st_src, itr_src). remember (st_tgt, itr_tgt).
 		
-		(* revert st_src st_tgt itr_src itr_tgt Heqp Heqp0 Heqt Heqt0 CIH. *)
-		revert mr_src mr_tgt fr_src fr_tgt FMR st_src st_tgt itr_src itr_tgt Heqp Heqp0 CIH.
-		(* revert mr_src mr_tgt fr_src fr_tgt FMR st_src st_tgt itr_src itr_tgt Heqp Heqp0 Heqt Heqt0 CIH. *)
+		revert mr_src mr_tgt fr_src fr_tgt FMR st_src st_tgt itr_src itr_tgt Heqp Heqp0 CIH WF.
 
 		induction SIM using hpsim_ind; i; clarify; unfold interp_hp_tgt_fun, handle_Guarantee, mget, mput.
 		- steps.
@@ -601,17 +618,133 @@ Qed.
 			steps. force_l. 
 			{ iIntros "H". et. } 
 			(* rr. uipropall. }  *)
+			steps. econs; esplits; et. econs. esplits; et.  *)
+
+
+	Inductive hpsim_adeq_rel : Σ -> Σ -> (itree hAGEs Any.t)-> (stateT Σ (itree Es) Any.t) ->  Σ -> Σ -> (itree hAGEs Any.t)-> (stateT Σ (itree Es) Any.t) -> Prop :=
+	| hpsim_adeq_base (fr mr fr' mr': Σ) st st'
+		: hpsim_adeq_rel fr mr (Ret st) (fun fr0 => '(fr1, _) <- (handle_Guarantee (True%I:iProp) fr0);; Ret (fr1, st))
+										 fr' mr' (Ret st') (fun fr0 => '(fr1, _) <- (handle_Guarantee (True%I:iProp) fr0);; Ret (fr1, st'))
+
+	| hpsim_adeq_seq itrH0 itrH1 itrL0 itrL1 itrH0' itrH1' itrL0' itrL1' (fr mr fr1 fr' mr' fr1': Σ)
+			(ITR0: itrL0 = @interp_hp_tgt_fun Σ Any.t itrH0)
+			(ITR0': itrL0' = @interp_hp_tgt_fun Σ Any.t itrH0')
+			(ADEQ: forall st st' (mr1 mr1': Σ), hpsim_adeq_rel fr1 mr1 (itrH1 st) (itrL1 st) 
+																												fr1' mr1' (itrH1' st') (itrL1' st'))
+		: hpsim_adeq_rel fr mr (st0 <- itrH0;; itrH1 st0) (fun fr0 => '(_, st1) <- (itrL0 fr0);; (itrL1 st1 fr1))
+										fr' mr' (st0 <- itrH0';; itrH1' st0) (fun fr0 => '(_, st1) <- (itrL0' fr0);; (itrL1' st1 fr1'))
+	.
+
+
+  Lemma hpsim_adequacy
+			(fl_src0 fl_tgt0: alist string (Any.t -> itree Es Any.t)) 
+			(FLS: fl_src0 = List.map (fun '(s, f) => (s, interp_hp_fun f)) fl_src)
+			(FLT: fl_tgt0 = List.map (fun '(s, f) => (s, interp_hp_fun f)) fl_tgt)
+			f_src f_tgt st_src st_tgt itrH_src itrH_tgt itrL_src itrL_tgt
+			(ctx mr_src mr_tgt fr_src fr_tgt fmr: Σ)
+      (SIM: hpsim f_src f_tgt (st_src, itrH_src) (st_tgt, itrH_tgt) fmr)
+			(WF: URA.wf (ctx ⋅ fr_src ⋅ mr_src))
+			(FMR: Own (fr_src ⋅ mr_src) ⊢ #=> Own (fmr ⋅ fr_tgt ⋅ mr_tgt))
+			(REL: hpsim_adeq_rel fr_src mr_src itrH_src itrL_src fr_tgt mr_tgt itrH_tgt itrL_tgt)
+		:
+
+			@sim_itree Σ (mk_inv I) eq fl_src0 fl_tgt0 f_src f_tgt ctx 
+			(Any.pair st_src mr_src↑, (itrL_src fr_src) >>= (fun r => Ret (snd r)))
+			(Any.pair st_tgt mr_tgt↑, (itrL_tgt fr_tgt) >>= (fun r => Ret (snd r))).
+  Proof.
+		revert_until FLT.
+		ginit. gcofix CIH. i.
+		move REL before CIH. revert_until REL. induction REL.
+		{ i. punfold SIM. inv SIM; (try rewrite ! bind_trigger in H3); (try rewrite ! bind_trigger in H5); clarify.
+			- steps. unfold handle_Guarantee, mput, mget, guarantee. steps.
+				force_l. instantiate (1:= (c0 ⋅ c1, ε, fmr ⋅ c)).
+				steps. force_l.
+				{  
+					rewrite FMR. 
+					iIntros "H". iMod "H".
+					rewrite <- URA.add_assoc. 
+					iDestruct "H" as "[H H0]".
+					iPoseProof (x with "H0") as "H0". iMod "H0". 
+					iModIntro. r_solve.
+					replace (c0 ⋅ c1 ⋅ fmr ⋅ c) with (c0 ⋅ c1 ⋅ c ⋅ fmr); r_solve.
+					iSplitR "H"; et.
+				}
+				steps. force_l; et.
+				steps.
+				econs; esplits; et. econs; esplits; et.
+				{  
+					eapply own_ctx in FMR. rewrite URA.add_assoc in FMR. eapply own_wf in FMR; et.
+					rewrite <- URA.add_assoc in FMR. rewrite URA.add_assoc in FMR.
+					eapply own_ctx, own_wf in x; et.
+					replace (ctx ⋅ fmr ⋅ (c0 ⋅ c1 ⋅ c)) with (ctx ⋅ fmr ⋅ c ⋅ (c0 ⋅ c1)) in x; r_solve.
+					eapply URA.wf_mon; et.
+				}
+			- pclearbot. punfold SIM0. inv SIM0; (try rewrite ! bind_trigger in H3); (try rewrite ! bind_trigger in H5); clarify.
+				steps. unfold handle_Guarantee, mput, mget, guarantee. steps.
+				force_l. instantiate (1:= (c0 ⋅ c1, ε, fmr ⋅ c)).
+				steps. force_l.
+				{  
+					rewrite FMR. 
+					iIntros "H". iMod "H".
+					rewrite <- URA.add_assoc. 
+					iDestruct "H" as "[H H0]".
+					iPoseProof (x with "H0") as "H0". iMod "H0". 
+					iModIntro. r_solve.
+					replace (c0 ⋅ c1 ⋅ fmr ⋅ c) with (c0 ⋅ c1 ⋅ c ⋅ fmr); r_solve.
+					iSplitR "H"; et.
+				}
+				steps. force_l; et.
+				steps.
+				econs; esplits; et. econs; esplits; et.
+				{  
+					eapply own_ctx in FMR. rewrite URA.add_assoc in FMR. eapply own_wf in FMR; et.
+					rewrite <- URA.add_assoc in FMR. rewrite URA.add_assoc in FMR.
+					eapply own_ctx, own_wf in x; et.
+					replace (ctx ⋅ fmr ⋅ (c0 ⋅ c1 ⋅ c)) with (ctx ⋅ fmr ⋅ c ⋅ (c0 ⋅ c1)) in x; r_solve.
+					eapply URA.wf_mon; et.
+				}
+		}
+		
+		remember (st_src, itrH_src) as sti_src. remember (st_tgt, itrH_tgt) as sti_tgt.
+		move SIM before CIH. revert_until SIM.
+		induction SIM using hpsim_ind; i; clarify; unfold interp_hp_tgt_fun, handle_Guarantee, mget, mput.
+
+		- steps.
+			force_l. instantiate (1 := (c0 ⋅ c1, ε, fmr ⋅ c)). steps.
+			unfold guarantee. force_l.
+			{ 
+				rewrite FMR. 
+				iIntros "H". iMod "H".
+				rewrite <- URA.add_assoc. 
+				iDestruct "H" as "[H1 H2]".
+				iPoseProof (_GUARANTEE with "H2") as "H2".
+				iMod "H2".
+				iModIntro. r_solve.
+				iDestruct "H2" as "[H3 H4]".
+				iSplitR "H4"; et.
+				iCombine "H3 H1" as "H". et.
+			} 
+			steps. force_l. 
+			{ iIntros "H". et. } 
 			steps. econs; esplits; et.
-			+ econs. esplits; et. 
-			+ admit.
+			+ econs. esplits; et.
+				eapply own_ctx with (ctx:= ctx ⋅ fmr) in _GUARANTEE.
+				eapply own_ctx with (ctx:= ctx) in FMR.
+				rewrite <- URA.add_assoc in WF. eapply own_wf in FMR; et.
+				rewrite ! URA.add_assoc in FMR.
+				rewrite URA.add_assoc in _GUARANTEE.
+				eapply own_wf in _GUARANTEE; et.
+				replace (ctx ⋅ fmr ⋅ (c0 ⋅ c1 ⋅ c)) with (ctx ⋅ (fmr ⋅ c) ⋅ c0 ⋅ c1) in _GUARANTEE. 2: { r_solve. }
+				do 2 eapply URA.wf_mon; et.
 		- hexploit INV. i.
-			eapply iProp_sepconj in H; et. 2: { admit. }
+			eapply iProp_sepconj in H. et.
 			des.
 			rename rq into fr. rename rp into mr.
 			steps.
 			unfold handle_Guarantee, mget, mput. steps_safe.
 			force_l.
 			instantiate (1:= (c0, fr ⋅ c1, mr ⋅ c)).
+			rename c1 into fr_tgt'. rename c into mr_tgt'.
 			steps_safe.
 			unfold guarantee. force_l.
 			{ 
@@ -619,39 +752,89 @@ Qed.
 				rewrite <- URA.add_assoc.
 				iDestruct "H" as "[H H0]". 
 				iPoseProof (H with "H") as "H".
-				replace (c0 ⋅ (fr ⋅ c1) ⋅ (mr ⋅ c)) with (mr ⋅ fr ⋅ (c0 ⋅ c1 ⋅ c)). 2: { r_solve. }
+				replace (c0 ⋅ (fr ⋅ fr_tgt') ⋅ (mr ⋅ mr_tgt')) with (mr ⋅ fr ⋅ (c0 ⋅ fr_tgt' ⋅ mr_tgt')). 2: { r_solve. }
 				iPoseProof (_GUARANTEE with "H0") as "H0".
 				iSplitL "H"; et.
 			}
 			steps_safe. force_l.
 			{ et. }
-			steps_safe.
-			{ econs. esplits; et. admit. }
-			inv WF. des.
-			unfold interp_hp_tgt_fun, handle_Guarantee, mget, mput, guarantee in K.
-			hexploit K. 
+			steps_safe. eapply safe_sim_sim; econs; i.
+			exists (fr ⋅ ctx). esplits.
 			{ 
-				instantiate (1:= st_tgt). instantiate (1:= st_src).
+				econs. esplits; et.
+				{
+					eapply own_ctx with (ctx:= ctx ⋅ fmr) in _GUARANTEE.
+					eapply own_ctx with (ctx:= ctx) in FMR.
+					rewrite <- URA.add_assoc in WF. eapply own_wf in FMR; et.
+					rewrite ! URA.add_assoc in FMR.
+					rewrite URA.add_assoc in _GUARANTEE.
+					eapply own_wf in _GUARANTEE; et.
+					rewrite URA.add_comm in _GUARANTEE. rewrite URA.add_assoc in _GUARANTEE.
+					eapply own_ctx in H. eapply own_wf in H; et.
+					replace (c0 ⋅ fr_tgt' ⋅ mr_tgt' ⋅ ctx ⋅ (mr ⋅ fr)) with (fr ⋅ ctx ⋅ mr ⋅ mr_tgt' ⋅ (c0 ⋅ fr_tgt')) in H; r_solve.
+					eapply URA.wf_mon; et.
+				} 
+				iIntros "H". iPoseProof (H0 with "H") as "H". et.
+			}
+			i. inv WF0. des.
+			unfold interp_hp_tgt_fun, handle_Guarantee, mget, mput, guarantee in K.
+			hexploit K; swap 1 2.
+			{ 
 				iIntros "[H1 H2]".
 				iPoseProof (H1 with "H1") as "H1". 
 				iPoseProof (MR with "H2") as "H2".
 				iSplitL "H2"; et.
 			}
+			{
+				eapply own_ctx in MRS. eapply own_wf in MRS; et.
+				replace (fr ⋅ ctx ⋅ (mr0 ⋅ mr_tgt0)) with (fr ⋅ mr0 ⋅ (ctx ⋅ mr_tgt0)) in MRS; r_solve.
+				eapply URA.wf_mon; et.				
+			}
 			i. des.
-			gstep. econs. gfinal. left. 
+			steps. 
 			unfold interp_hp_tgt_fun, handle_Guarantee, mget, mput in *. rewrite <- ! bind_bind in *.
-			eapply CIH; et.
-			{ eapply hpsim_bot_flag_up. et. }
+			eapply IH; et.
 			{ 
 				iIntros "[H H0]".
 				iPoseProof (MRS with "H0") as "H0".
-				replace (fr ⋅ mr0 ⋅ c1 ⋅ mr_tgt0) with (fr ⋅ c1 ⋅ (mr0 ⋅ mr_tgt0)). 2: { r_solve. }  
+				replace (fr ⋅ mr0 ⋅ fr_tgt' ⋅ mr_tgt0) with (fr ⋅ fr_tgt' ⋅ (mr0 ⋅ mr_tgt0)). 2: { r_solve. }  
 				iSplitL "H"; et.
+			}
+			{
+				clear IH.
+
+				admit.	
 			}
 		- steps. hexploit K; et. i. des.
 			unfold interp_hp_tgt_fun, handle_Guarantee, mget, mput in *. rewrite <- ! bind_bind in *.
 			eapply IH; et.
-		- admit. (* need to clarify the relation between fl_src ~ fl_src0 *)
+		- steps. unfold handle_Guarantee, mget, mput, guarantee. steps.
+			force_l.
+			instantiate (1:= (ε, ε, fr_src ⋅ mr_src)).
+			steps. force_l. { r_solve. et. }
+			steps. force_l; et. 
+			steps. 
+			{ 
+				instantiate (1:= interp_hp_fun f).
+				rewrite alist_find_map. rewrite FUN. et.
+			}
+			unfold interp_hp_fun, interp_hp_tgt_fun. steps.
+			do 3 rewrite <- bind_bind in *.
+			(* set (` x : Σ * Any.t <- interp_hp_tgt (f varg) ε;; (let '(_, x0) := x in Ret x0)) as itr. *)
+			(* assert () *)
+			set ((` x : Σ * Any.t <- (` x : Any.t <- (` x : Σ * Any.t <- interp_hp_tgt (f varg) ε;; (let '(_, x0) := x in Ret x0));; (tau;; Ret (fr_src, x)));;
+			interp_hp_tgt (k_src x.2) x.1)) as itr0.
+			set (interp_hp_tgt (` x : Any.t <- (f varg);; k_src x) fr_src) as itr1.
+			assert (itr0 = itr1 ). {
+				unfold itr0, itr1. grind. rewrite interp_hp_bind.	
+			admit. }
+			rewrite H. unfold itr1.
+			(* assert (itr_src = interp_hp_tgt (` x : Any.t <- (f varg);; ` x : Σ * Any.t <- (k_src x)) fr_src).
+			{ unfold itr_src. grind. }
+			rewrite <- interp_hp_bind. *)
+			unfold interp_hp_tgt_fun, handle_Guarantee, mget, mput in *. rewrite <- ! bind_bind in *.
+			eapply IHSIM; et.
+	
 		- admit. 
 		- steps. unfold interp_hp_tgt_fun, handle_Guarantee, mget, mput in *. rewrite <- ! bind_bind in *. et.
 		- steps. unfold interp_hp_tgt_fun, handle_Guarantee, mget, mput in *. rewrite <- ! bind_bind in *. et.
@@ -665,70 +848,79 @@ Qed.
 		- steps. force_r. steps. unfold interp_hp_tgt_fun, handle_Guarantee, mget, mput in *. rewrite <- ! bind_bind in *. et.
 		- steps. rewrite ! Any.pair_split. rewrite RUN. s.
 			unfold interp_hp_tgt_fun, handle_Guarantee, mget, mput in *. rewrite <- ! bind_bind in *.
-			exploit IHSIM; et.
+			eapply IHSIM; et.
 		- steps. rewrite ! Any.pair_split. rewrite RUN. s.
 			unfold interp_hp_tgt_fun, handle_Guarantee, mget, mput in *. rewrite <- ! bind_bind in *.
-			exploit IHSIM; et.
+			eapply IHSIM; et.
 		- steps. rewrite interp_hp_Assume. unfold handle_Assume, mget, mput. steps.  
 			unfold interp_hp_tgt_fun, handle_Guarantee, mget, mput in *. rewrite <- ! bind_bind in *.
-			hexploit K; et.
+			(* hexploit K. *)
+			hexploit (K (x ⋅ fmr)). et.
 			{ 
-				instantiate (1:= x ⋅ fmr).
+				eapply own_ctx in FMR0. eapply own_wf in FMR0; cycle 1.
+				{ rewrite URA.add_assoc; et.  }
+				{ rewrite ! URA.add_assoc in FMR0. do 2 eapply URA.wf_mon; et.  }
+			}
+			et.
+			{
 				iIntros "[H H0]". 
 				iPoseProof (_ASSUME0 with "H") as "H".
 				iPoseProof (CUR with "H0") as "H0".
 				iMod "H0". iModIntro. iFrame. 
 			}
 			i. des. eapply IH; et.
-			rewrite <- ! URA.add_assoc.
 			{
+				rewrite <- ! URA.add_assoc.
 				iIntros "[H H0]".
 				iSplitL "H"; et.
 				iPoseProof (FMR0 with "H0") as "H".
 				rewrite URA.add_assoc. et.
 			}
+			{
+				clear IH. admit.
+			}
 		-	steps. rewrite interp_hp_Assume. 
 			hexploit CUR. i.
-			apply iProp_sepconj in H. 2: { admit. }
+			apply iProp_sepconj in H.
 			des. rename rq into fmr0.
 			unfold handle_Assume, mget, mput, assume. steps.
 			force_r.
 			instantiate (1:= rp).
 			steps. force_r.
 			{ 
-				clear -H FMR0.
-				assert (URA.wf (fmr ⋅ fr_tgt ⋅ mr_tgt)). { admit. }
-				assert (URA.wf (fmr ⋅ fr_tgt ⋅ mr_tgt ⋅ ε)). { admit. }
-				eapply own_ctx with (ctx := (fr_tgt ⋅ mr_tgt)) in H.
-				uipropall.
-				eapply H in H0. 2: { admit. }
-				des.
-				eapply URA.wf_extends in H0. admit.
-				specialize (H2 ε H1).
-				admit.
+				eapply own_ctx in FMR0. rewrite URA.add_assoc in FMR0. eapply own_wf in FMR0; et.
+				replace (ctx ⋅ (fmr ⋅ fr_tgt ⋅ mr_tgt)) with (ctx ⋅ fr_tgt ⋅ mr_tgt ⋅ fmr) in FMR0; r_solve.
+				eapply own_ctx in H. eapply own_wf in H; et.
+				replace (ctx ⋅ fr_tgt ⋅ mr_tgt ⋅ (rp ⋅ fmr0)) with (rp ⋅ fr_tgt ⋅ mr_tgt ⋅ (ctx ⋅ fmr0)) in H; r_solve.
+				eapply URA.wf_mon; et.	
 			}
-
 			steps. force_r; et. 
 			steps.
 			unfold interp_hp_tgt_fun, handle_Guarantee, mget, mput in *. rewrite <- ! bind_bind in *.
-			hexploit K; et. 
+			hexploit (K fmr0).
 			{
+				eapply own_ctx in FMR0. rewrite URA.add_assoc in FMR0; et. eapply own_wf in FMR0; et.
+				replace (ctx ⋅ (fmr ⋅ fr_tgt ⋅ mr_tgt )) with (fmr ⋅ (ctx ⋅ fr_tgt ⋅ mr_tgt)) in FMR0; r_solve.
+				eapply URA.wf_mon in FMR0. eapply own_wf in H; et.
+				rewrite URA.add_comm in H. eapply URA.wf_mon; et.
+			}
+			{ 
 				iIntros "H". iPoseProof (H1 with "H") as "H". et.
 			}
-			i. des. 
+			i. des.
 			eapply IH; et.
 			{
-				iIntros "H". 
-				iPoseProof (FMR0 with "H") as "H". iMod "H". rewrite <- ! URA.add_assoc.
-				iDestruct "H" as "[H H0]".
-				replace (fmr0 ⋅ (rp ⋅ (fr_tgt ⋅ mr_tgt))) with ((rp ⋅ fmr0) ⋅ (fr_tgt ⋅ mr_tgt)). 2: { r_solve. }
+				clear IH.
+				iIntros "H". iPoseProof (FMR0 with "H") as "H".
+				rewrite <- URA.add_assoc. iMod "H". iDestruct "H" as "[H H0]".
+				r_solve. rewrite <- URA.add_assoc. iSplitL "H"; et.
 				iPoseProof (H with "H") as "H". iMod "H".
-				iSplitL "H"; et.
-			} 
+				iDestruct "H" as "[H H0]". iSplitL "H0"; et.  				
+			}
 		- steps. rewrite interp_hp_Guarantee.
 			unfold handle_Guarantee, mget, mput, guarantee. steps.
 			hexploit CUR. i.
-			apply iProp_sepconj in H.  2: { admit. }
+			apply iProp_sepconj in H.
 			des. rename rq into fmr0.
 			force_l.
 			instantiate (1:= (rp, fr_tgt, fmr0 ⋅ mr_tgt)).
@@ -744,7 +936,14 @@ Qed.
 			}
 			steps. force_l; et.
 			steps.
-			hexploit K; et.
+			hexploit (K fmr0); et.
+			{
+				eapply own_ctx in FMR0. rewrite URA.add_assoc in FMR0. eapply own_wf in FMR0; et.
+				replace (ctx ⋅ (fmr ⋅ fr_tgt ⋅ mr_tgt)) with (ctx ⋅ fr_tgt ⋅ mr_tgt ⋅ fmr) in FMR0; r_solve.
+				eapply own_ctx, own_wf in H; et.
+				rewrite URA.add_assoc in H.
+				eapply URA.wf_mon. rewrite URA.add_comm. et.
+			}
 			{
 				iIntros "H". iPoseProof (H1 with "H") as "H". et.	
 			}
@@ -755,11 +954,25 @@ Qed.
 				replace (fr_tgt ⋅ (fmr0 ⋅ mr_tgt)) with (fmr0 ⋅ fr_tgt ⋅ mr_tgt); r_solve.
 				et.
 			}
+			{
+				clear IH. 
+				eapply own_ctx in FMR0. rewrite URA.add_assoc in FMR0. eapply own_wf in FMR0; et.
+				replace (ctx ⋅ (fmr ⋅ fr_tgt ⋅ mr_tgt)) with (ctx ⋅ fr_tgt ⋅ mr_tgt ⋅ fmr) in FMR0; r_solve.
+				eapply own_ctx, own_wf in H; et.
+				replace (ctx ⋅ fr_tgt ⋅ mr_tgt ⋅ (rp ⋅ fmr0)) with (ctx ⋅ fr_tgt ⋅ fmr0 ⋅ mr_tgt ⋅ rp) in H; r_solve.
+				eapply URA.wf_mon; et.
+			}
 		- steps. rewrite interp_hp_Guarantee. unfold handle_Guarantee, mget, mput, guarantee. steps. 
 			unfold interp_hp_tgt_fun, handle_Guarantee, mget, mput in *. rewrite <- ! bind_bind in *.			
-			hexploit K; et.
+			hexploit (K (c0 ⋅ fmr)). 
+			{
+				eapply own_ctx in FMR0. rewrite URA.add_assoc in FMR0. eapply own_wf in FMR0; et.
+				rewrite <- URA.add_assoc in FMR0. rewrite URA.add_assoc in FMR0.
+				eapply own_ctx, own_wf in x; et.
+				replace (ctx ⋅ fmr ⋅ (c0 ⋅ c1 ⋅ c)) with (c0 ⋅ fmr ⋅ (ctx ⋅ c1 ⋅ c)) in x; r_solve.
+				eapply URA.wf_mon; et.
+			}
 			{ 
-				instantiate (1:= (c0 ⋅ fmr)).
 				iIntros "[H H0]".
 				iPoseProof (x0 with "H") as "H".
 				iPoseProof (CUR with "H0") as "H0".
@@ -777,8 +990,6 @@ Qed.
 				iSplitL "H"; et.
 			}
 		- gstep. econs. gfinal. left. eapply CIH; et. 
-		
-			(* (fr_src ⋅ mr_src) -> fmr in 'SIM' *)
 	Admitted.
 
 
